Finish proc_indexed_interp_unguarded_weak_norm

Wavelet/Dataflow/EqMod.lean
@@ -27,46 +27,153 @@ theorem ChanMap.EqMod.eq_eq {map₁ map₂ : ChanMap χ V} :
   · intros h
     simp [h, EqMod]
 
+def AsyncOp.EqMod
+  (EqV : V → V → Prop) :
+    AsyncOp V → AsyncOp V → Prop
+  | .const c₁ n₁, .const c₂ n₂ => EqV c₁ c₂ ∧ n₁ = n₂
+  | .forwardc n₁ m₁ consts₁, .forwardc n₂ m₂ consts₂ =>
+      n₁ = n₂ ∧ m₁ = m₂ ∧ List.Forall₂ EqV consts₁.toList consts₂.toList
+  | aop₁, aop₂ => aop₁ = aop₂
+
+def AtomicProc.EqMod
+  [Arity Op]
+  (EqV : V → V → Prop) : AtomicProc Op χ V → AtomicProc Op χ V → Prop
+  | .async aop₁ inputs₁ outputs₁, .async aop₂ inputs₂ outputs₂ =>
+    AsyncOp.EqMod EqV aop₁ aop₂ ∧
+    inputs₁ = inputs₂ ∧
+    outputs₁ = outputs₂
+  | ap₁, ap₂ => ap₁ = ap₂
+
+def Proc.EqMod
+  [Arity Op]
+  (EqV : V → V → Prop)
+  (p₁ p₂ : Proc Op χ V m n) : Prop :=
+  p₁.inputs = p₂.inputs ∧
+  p₁.outputs = p₂.outputs ∧
+  List.Forall₂ (AtomicProc.EqMod EqV) p₁.atoms p₂.atoms
+
 /-- Equal configurations modulo a equivalence relation on values. -/
 def Config.EqMod
-  [Arity Op] (Eq : V → V → Prop)
+  [Arity Op] (EqV : V → V → Prop)
   (c₁ c₂ : Config Op χ V m n) : Prop :=
-  c₁.proc = c₂.proc ∧
-  ChanMap.EqMod Eq c₁.chans c₂.chans
+  Proc.EqMod EqV c₁.proc c₂.proc ∧
+  ChanMap.EqMod EqV c₁.chans c₂.chans
 
-instance {Eq : V → V → Prop} [Arity Op] [IsRefl V Eq] :
-  IsRefl (Config Op χ V m n) (Config.EqMod Eq) where
-  refl c := by
-    constructor
-    · rfl
-    · apply IsRefl.refl
+instance {EqV : V → V → Prop} [IsRefl V EqV] :
+  IsRefl (AsyncOp V) (AsyncOp.EqMod EqV) where
+  refl := sorry
 
-instance {Eq : V → V → Prop} [Arity Op] [IsSymm V Eq] :
-  IsSymm (Config Op χ V m n) (Config.EqMod Eq) where
+instance {EqV : V → V → Prop} [IsSymm V EqV] :
+  IsSymm (AsyncOp V) (AsyncOp.EqMod EqV) where
   symm := sorry
 
-instance {Eq : V → V → Prop} [Arity Op] [IsTrans V Eq] :
-  IsTrans (Config Op χ V m n) (Config.EqMod Eq) where
+instance {EqV : V → V → Prop} [IsTrans V EqV] :
+  IsTrans (AsyncOp V) (AsyncOp.EqMod EqV) where
+  trans := sorry
+
+instance {EqV : V → V → Prop} [Arity Op] [IsRefl V EqV] :
+  IsRefl (AtomicProc Op χ V) (AtomicProc.EqMod EqV) where
+  refl := sorry
+
+instance {EqV : V → V → Prop} [Arity Op] [IsSymm V EqV] :
+  IsSymm (AtomicProc Op χ V) (AtomicProc.EqMod EqV) where
+  symm := sorry
+
+instance {EqV : V → V → Prop} [Arity Op] [IsTrans V EqV] :
+  IsTrans (AtomicProc Op χ V) (AtomicProc.EqMod EqV) where
+  trans := sorry
+
+instance {EqV : V → V → Prop} [Arity Op] [IsRefl V EqV] :
+  IsRefl (Proc Op χ V m n) (Proc.EqMod EqV) where
+  refl := sorry
+
+instance {EqV : V → V → Prop} [Arity Op] [IsSymm V EqV] :
+  IsSymm (Proc Op χ V m n) (Proc.EqMod EqV) where
+  symm := sorry
+
+instance {EqV : V → V → Prop} [Arity Op] [IsTrans V EqV] :
+  IsTrans (Proc Op χ V m n) (Proc.EqMod EqV) where
+  trans := sorry
+
+instance {EqV : V → V → Prop} [Arity Op] [IsRefl V EqV] :
+  IsRefl (Config Op χ V m n) (Config.EqMod EqV) where
+  refl := sorry
+
+instance {EqV : V → V → Prop} [Arity Op] [IsSymm V EqV] :
+  IsSymm (Config Op χ V m n) (Config.EqMod EqV) where
+  symm := sorry
+
+instance {EqV : V → V → Prop} [Arity Op] [IsTrans V EqV] :
+  IsTrans (Config Op χ V m n) (Config.EqMod EqV) where
   trans := sorry
 
 @[simp]
-theorem Config.EqMod.eq_eq
-  [Arity Op] {c₁ c₂ : Config Op χ V m n} :
-    Config.EqMod Eq c₁ c₂ ↔ c₁ = c₂
-  := by
+theorem AsyncOp.EqMod.eq_eq : AsyncOp.EqMod Eq = Eq (α := AsyncOp V) := by
+  funext
   simp [EqMod]
-  cases c₁; cases c₂
-  simp
+  split
+  · simp
+  · constructor
+    · intros h
+      have ⟨h₁, h₂, h₃⟩ := h
+      subst h₁; subst h₂
+      simp [Vector.toList_inj] at h₃
+      simp [h₃]
+    · intros h
+      simp at h
+      have ⟨h₁, h₂, h₃⟩ := h
+      subst h₁; subst h₂; subst h₃
+      simp
+  · simp
+
+@[simp]
+theorem AtomicProc.EqMod.eq_eq
+  [Arity Op] : AtomicProc.EqMod Eq = Eq (α := AtomicProc Op χ V)
+  := by
+  funext
+  simp [EqMod]
+  split <;> simp
+
+@[simp]
+theorem Proc.EqMod.eq_eq
+  [Arity Op] : Proc.EqMod Eq = Eq (α := Proc Op χ V m n)
+  := by
+  funext p₁ p₂
+  cases p₁
+  cases p₂
+  simp [EqMod]
+
+@[simp]
+theorem Config.EqMod.eq_eq
+  [Arity Op] : Config.EqMod Eq = Eq (α := Config Op χ V m n)
+  := by
+  funext c₁ c₂
+  cases c₁
+  cases c₂
+  simp [EqMod]
+
+theorem chan_map_pop_vals_equiv
+  [DecidableEq χ]
+  {map₁ map₂ : ChanMap χ V}
+  {vals₁ : Vector V k}
+  {EqV : V → V → Prop}
+  (heq : ChanMap.EqMod EqV map₁ map₂)
+  (hpop : map₁.popVals names = some (vals₁, map₁')) :
+    ∃ vals₂ map₂',
+      map₂.popVals names = some (vals₂, map₂') ∧
+      List.Forall₂ EqV vals₁.toList vals₂.toList ∧
+      ChanMap.EqMod EqV map₁' map₂'
+  := sorry
 
 theorem chan_map_push_vals_equiv
   [DecidableEq χ]
   {map : ChanMap χ V}
   {vals₁ vals₂ : Vector V k}
-  {Eq : V → V → Prop}
-  (hequiv : List.Forall₂ Eq vals₁.toList vals₂.toList) :
+  {EqV : V → V → Prop}
+  (hequiv : List.Forall₂ EqV vals₁.toList vals₂.toList) :
     ChanMap.EqMod EqV
-      (ChanMap.pushVals names vals₁ map)
-      (ChanMap.pushVals names vals₂ map)
+      (map.pushVals names vals₁)
+      (map.pushVals names vals₂)
   := sorry
 
 end Wavelet.Dataflow
